src/FramePreservationValidator.v
@@ -9,6 +9,7 @@ Require Import TransformContract.
 Require Import StateView.
 Require Import ViewPipeline.
 Require Import FramePreservationWitness.
+Require Import FrameValueWitness.
 
 Import ListNotations.
 
@@ -63,6 +64,20 @@ Record frame_preservation_view_contract
       input_view output_view source_view after;
 }.
 
+Record frame_preservation_value_view_contract
+    (value: Type)
+    (input_view output_view: View.view)
+    (frame_cells write_cells allowed_write_cells: list MemCell)
+    (frame_entries: list (frame_value_entry value))
+    (source_view after: PolyLang.t) : Prop := {
+  fpvvc_frame_contract :
+    frame_preservation_view_contract
+      input_view output_view frame_cells write_cells allowed_write_cells
+      source_view after;
+  fpvvc_frame_values :
+    frame_value_obligations value frame_cells frame_entries;
+}.
+
 Definition frame_pipeline_final_view
     (output_view: View.view) : View.view :=
   Pipeline.pipeline_final_view output_view.
@@ -100,6 +115,67 @@ Proof.
       (Pipeline.compose_checked_source_view
          input_view output_view before source_view after ok);
       assumption.
+Qed.
+
+Theorem checked_frame_preservation_value_view_correct :
+  forall (value: Type) (value_eqb: value -> value -> bool)
+         input_view output_view frame_cells write_cells allowed_write_cells
+         frame_entries before source_view after ok,
+    (forall left right,
+        value_eqb left right = true ->
+        left = right) ->
+    mayReturn (check_frame_source_view before source_view) ok ->
+    ok = true ->
+    check_frame_preservationb
+      frame_cells write_cells allowed_write_cells = true ->
+    check_frame_valueb value value_eqb frame_cells frame_entries = true ->
+    frame_source_view_refines_view
+      input_view output_view source_view after ->
+    frame_preservation_value_view_contract
+      value input_view output_view
+      frame_cells write_cells allowed_write_cells frame_entries
+      source_view after /\
+    View.view_refinement
+      input_view
+      (frame_pipeline_final_view output_view)
+      before after.
+Proof.
+  intros value value_eqb input_view output_view frame_cells write_cells
+         allowed_write_cells frame_entries before source_view after ok
+         Hvalue_eqb Hret Hok Hframe Hvalues Hsemantics.
+  pose proof
+    (checked_frame_preservation_view_correct
+       input_view output_view frame_cells write_cells allowed_write_cells
+       before source_view after ok Hret Hok Hframe Hsemantics)
+    as [Hframe_contract Hrefinement].
+  pose proof
+    (check_frame_valueb_sound
+       value value_eqb Hvalue_eqb frame_cells frame_entries Hvalues)
+    as Hvalue_obligations.
+  split.
+  - constructor; assumption.
+  - exact Hrefinement.
+Qed.
+
+Theorem frame_preservation_frame_cell_value_preserved :
+  forall (value: Type) input_view output_view
+         frame_cells write_cells allowed_write_cells frame_entries
+         source_view after cell,
+    frame_preservation_value_view_contract
+      value input_view output_view
+      frame_cells write_cells allowed_write_cells frame_entries
+      source_view after ->
+    In cell frame_cells ->
+    exists entry,
+      In entry frame_entries /\
+      fve_frame_cell entry = cell /\
+      fve_before_value entry = fve_after_value entry.
+Proof.
+  intros value input_view output_view frame_cells write_cells
+         allowed_write_cells frame_entries source_view after cell
+         Hcontract Hin.
+  destruct Hcontract as [_ Hvalues].
+  eapply frame_value_cell_preserved; eauto.
 Qed.
 
 End FramePreservationValidator.
